cti/Coq: Adapt eval from dev-coq source

cti/BaseFix.v
@@ -1,5 +1,5 @@
 Require Import String Arith List.
-Import ListNotations.
+Import ListNotations IfNotations.
 
 (* λ⇅ multi-level core language *)
 
@@ -17,7 +17,13 @@ Inductive op2 :=
   | OEq.
 
 Inductive error :=
-  | ErrUnboundVar.
+  | ErrUnboundVar
+  | ErrExpectedCode
+  | ErrIfExpectedNat
+  | ErrAppExpectedClo
+  | ErrInvalidOp
+  | ErrStage
+  | ErrExceededDepth.
 
 Inductive exp :=
   | ENat (n : nat)
@@ -66,45 +72,206 @@ Fixpoint anf (s : state) (ρ : list exp) (e : exp) : state * exp :=
   | ENat n => (s, ENat n)
   | EStr t => (s, EStr t)
   | ECons e0 e1 =>
-      let (s0, v0) := anf s ρ e0 in
-      let (s1, v1) := anf s0 ρ e1 in
-      reflect s1 (ECons v0 v1)
+      let (s, v0) := anf s ρ e0 in
+      let (s, v1) := anf s ρ e1 in
+      reflect s (ECons v0 v1)
   | ELam e0 =>
       let (s0, v0) := fresh s in
       let (s1, v1) := fresh s0 in
       reflect (fst s, snd s1)
               (ELam (reify (anf (fst s1, []) (v1 :: v0 :: ρ) e0)))
   | ELet e0 e1 =>
-      let (s0, v0) := anf s ρ e0 in
-      anf s0 (v0 :: ρ) e1
+      let (s, v0) := anf s ρ e0 in
+      anf s (v0 :: ρ) e1
   | EVar x => (s, lookup_exp ρ x)
   | EIf e0 e1 e2 =>
-      let (s0, v0) := anf s ρ e0 in
-      reflect s0 (EIf v0 (reify (anf (fst s0, []) ρ e1))
-                         (reify (anf (fst s0, []) ρ e2)))
+      let (s, v0) := anf s ρ e0 in
+      reflect s (EIf v0 (reify (anf (fst s, []) ρ e1))
+                        (reify (anf (fst s, []) ρ e2)))
   | EApp e0 e1 =>
-      let (s0, v0) := anf s ρ e0 in
-      let (s1, v1) := anf s0 ρ e1 in
-      reflect s1 (EApp v0 v1)
+      let (s, v0) := anf s ρ e0 in
+      let (s, v1) := anf s ρ e1 in
+      reflect s (EApp v0 v1)
   | EOp1 op e0 =>
-      let (s0, v0) := anf s ρ e0 in
-      reflect s0 (EOp1 op v0)
+      let (s, v0) := anf s ρ e0 in
+      reflect s (EOp1 op v0)
   | EOp2 op e0 e1 =>
-      let (s0, v0) := anf s ρ e0 in
-      let (s1, v1) := anf s0 ρ e1 in
-      reflect s1 (EOp2 op v0 v1)
+      let (s, v0) := anf s ρ e0 in
+      let (s, v1) := anf s ρ e1 in
+      reflect s (EOp2 op v0 v1)
   | ELift e0 =>
-      let (s0, v0) := anf s ρ e0 in
-      reflect s0 (ELift v0)
+      let (s, v0) := anf s ρ e0 in
+      reflect s (ELift v0)
   | ERun e0 e1 =>
-      let (s0, v0) := anf s ρ e0 in
-      let (s1, v1) := anf s0 ρ e1 in
-      reflect s1 (ERun v0 v1)
+      let (s, v0) := anf s ρ e0 in
+      let (s, v1) := anf s ρ e1 in
+      reflect s (ERun v0 v1)
   | EErr err => (s, e)
   end.
 
-Definition anf0 (e : exp) := reify (anf (0, []) [] e).
+Definition anf0 (e : exp) : exp :=
+  reify (anf (0, []) [] e).
 
-Example example_anf0 :
-  anf0 (ELam (EVar 1)) = ELet (ELam (EVar 1)) (EVar 0).
-Proof. reflexivity. Qed.
+Definition reifyc (sv : state * val) : exp :=
+  match sv with
+  | (s, VCode e0) => reify (s, e0)
+  | (_, VErr err) => EErr err
+  | _ => EErr ErrExpectedCode
+  end.
+
+Definition reflectc (s : state) (e : exp) : state * val :=
+  match reflect s e with
+  | (s, EErr err) => (s, VErr err)
+  | (s, v0) => (s, VCode v0)
+  end.
+
+Definition reifyv (sv : state * val) : val :=
+  match sv with
+  | ((_, []), v) => v
+  | (s, VCode e0) => VCode (reify (s, e0))
+  | (s, VErr err) => VErr err
+  | _ => VErr ErrExpectedCode
+  end.
+
+Fixpoint eval (depth : nat) (s : state) (ρ : list val) (e : exp) : state * val :=
+  match depth with
+  | 0 => (s, VErr ErrExceededDepth)
+  | S depth =>
+      match e with
+      | ENat n => (s, VNat n)
+      | EStr t => (s, VStr t)
+      | ECons e0 e1 =>
+          let (s, v0) := eval depth s ρ e0 in
+          if v0 is VErr err then (s, VErr err) else
+          let (s, v1) := eval depth s ρ e1 in
+          if v1 is VErr err then (s, VErr err) else
+          (s, VPair v0 v1)
+      | ELam e0 => (s, VClo ρ e0)
+      | ELet e0 e1 =>
+          let (s, v0) := eval depth s ρ e0 in
+          if v0 is VErr err then (s, VErr err) else
+          eval depth s (v0 :: ρ) e1
+      | EVar n => (s, lookup_val ρ n)
+      | EIf e0 e1 e2 =>
+          let (s, v0) := eval depth s ρ e0 in
+          match v0 with
+          | VErr err => (s, VErr err)
+          | VNat 0 => eval depth s ρ e2
+          | VNat _ => eval depth s ρ e1
+          | VCode v0 =>
+              match eval depth (fst s, []) ρ e1,
+                    eval depth (fst s, []) ρ e2 with
+              | (_, VErr err), _ | _, (_, VErr err) => (s, VErr err)
+              | r1, r2 => reflectc s (EIf v0 (reifyc r1) (reifyc r2))
+              end
+          | _ => (s, VErr ErrIfExpectedNat)
+          end
+      | EApp e0 e1 =>
+          let (s, v0) := eval depth s ρ e0 in
+          match v0 with
+          | VErr err => (s, VErr err)
+          | VClo ρ0 e0 =>
+              let (s, v2) := eval depth s ρ e1 in
+              if v2 is VErr err then (s, VErr err) else
+              eval depth s (v2 :: VClo ρ0 e0 :: ρ0) e0
+          | VCode e0 =>
+              let (s, v2) := eval depth s ρ e1 in
+              match v2 with
+              | VErr err => (s, VErr err)
+              | VCode e2 => reflectc s (EApp e0 e2)
+              | _ => (s, VErr ErrExpectedCode)
+              end
+          | _ => (s, VErr ErrAppExpectedClo)
+          end
+      | EOp1 op e0 =>
+          let (s, v0) := eval depth s ρ e0 in
+          match op, v0 with
+          | _, VErr err => (s, VErr err)
+          | _, VCode v0 => reflectc s (EOp1 op v0)
+          | OCar, VPair v0 v1 => (s, v0)
+          | OCdr, VPair v0 v1 => (s, v1)
+          | OIsNat, VNat _ => (s, VNat 1)
+          | OIsNat, _ => (s, VNat 0)
+          | OIsStr, VStr _ => (s, VNat 1)
+          | OIsStr, _ => (s, VNat 0)
+          | OIsPair, VPair _ _ => (s, VNat 1)
+          | OIsPair, _ => (s, VNat 0)
+          | _, _ => (s, VErr ErrInvalidOp)
+          end
+      | EOp2 op e0 e1 =>
+          let (s, v0) := eval depth s ρ e0 in
+          let (s, v1) := eval depth s ρ e1 in
+          match op, v0, v1 with
+          | _, VErr err, _ | _, _, VErr err => (s, VErr err)
+          | _, VCode v0, VCode v1 => reflectc s (EOp2 op v0 v1)
+          | _, VCode _, _ | _, _, VCode _ => (s, VErr ErrStage)
+          | OAdd, VNat n0, VNat n1 => (s, VNat (n0 + n1))
+          | OSub, VNat n0, VNat n1 => (s, VNat (n0 - n1))
+          | OMul, VNat n0, VNat n1 => (s, VNat (n0 * n1))
+          | OEq, VNat n0, VNat n1 => (s, VNat (if (n0 =? n1)%nat then 1 else 0))
+          | OEq, VStr t0, VStr t1 => (s, VNat (if (t0 =? t1)%string then 1 else 0))
+          | OEq, _, _ => (s, VNat 0)
+          | _, _, _ => (s, VErr ErrInvalidOp)
+          end
+      | ELift e0 =>
+          let (s, v0) := eval depth s ρ e0 in
+          if v0 is VErr err then (s, VErr err) else
+          let (s, v1) := lift depth s v0 in
+          if v1 is EErr err then (s, VErr err) else
+          (s, VCode v1)
+      | ERun e0 e1 =>
+          let (s0, v0) := eval depth s ρ e0 in
+          match v0 with
+          | VErr err => (s0, VErr err)
+          | VCode v0 =>
+              let (s1, v1) := eval depth (fst s0, []) ρ e1 in
+              if v1 is VErr err then (s1, VErr err) else
+              reflectc s0 (ERun v0 (reifyc (s1, v1)))
+          | _ =>
+              (s0, reifyv (eval depth (fst s0, []) ρ
+                                (reifyc (eval depth (length ρ, snd s0) ρ e1))))
+          end
+      | EErr err => (s, VErr err)
+      end
+    end
+
+with lift (depth : nat) (s : state) (v : val) : state * exp :=
+  match depth with
+  | 0 => (s, EErr ErrExceededDepth)
+  | S depth =>
+      match v with
+      | VNat n => (s, ENat n)
+      | VStr t => (s, EStr t)
+      | VPair v0 v1 =>
+          match v0, v1 with
+          | VCode e0, VCode e1 => reflect s (ECons e0 e1)
+          | VCode _, _ | _, VCode _ => (s, EErr ErrStage)
+          | _, _ => (s, EErr ErrExpectedCode)
+          end
+      | VClo ρ e0 =>
+          let (s0, v0) := fresh s in
+          let (s1, v1) := fresh s0 in
+          let (s2, v2) := eval depth (fst s1, []) (VCode v1 :: VCode v0 :: ρ) e0 in
+          match v2 with
+          | VErr err => (s0, EErr err)
+          | VCode e2 => reflect (fst s, snd s1) (ELam (reify (s2, e2)))
+          | _ => (s0, EErr ErrExpectedCode)
+          end
+      | VCode e0 => reflect s (ELift e0)
+      | VErr err => (s, EErr err)
+      end
+  end.
+
+Definition eval0 (e : exp) : state * val :=
+  eval 100 (0, []) [] e.
+
+Example ex0 : eval0 (ELam (EVar 1))                                  = ((0, []), VClo [] (EVar 1)).                                   reflexivity. Qed.
+Example ex1 : eval0 (anf0 (ELam (EVar 1)))                           = ((0, []), VClo [] (EVar 1)).                                   reflexivity. Qed.
+Example ex2 : eval0 (ELam (ELam (EVar 1)))                           = ((0, []), VClo [] (ELam (EVar 1))).                            reflexivity. Qed.
+Example ex3 : eval0 (anf0 (ELam (ELam (EVar 1))))                    = ((0, []), VClo [] (ELet (ELam (EVar 1)) (EVar 2))).            reflexivity. Qed.
+Example ex4 : reifyc (eval0 (ELift (ELam (EVar 1))))                 = ELet (ELam (EVar 1)) (EVar 0).                                 reflexivity. Qed.
+Example ex5 : anf0 (ELam (EVar 1))                                   = ELet (ELam (EVar 1)) (EVar 0).                                 reflexivity. Qed.
+Example ex6 : reifyc (eval0 (ELift (ELam (ELift (ELam (EVar 1))))))  = ELet (ELam (ELet (ELam (EVar 1)) (EVar 2))) (EVar 0).          reflexivity. Qed.
+Example ex7 : anf0 (ELam (ELam (EVar 1)))                            = ELet (ELam (ELet (ELam (EVar 1)) (EVar 2))) (EVar 0).          reflexivity. Qed.
+Example ex8 : eval0 (ERun (ELam (EVar 1)) (ELift (ELam (EVar 1))))   = ((0, []), VClo [] (EVar 1)).                                   reflexivity. Qed.
+Example ex9 : reifyc (eval0 (ELift (ELam (EApp (EVar 0) (EVar 1))))) = ELet (ELam (ELet (EApp (EVar 0) (EVar 1)) (EVar 2))) (EVar 0). reflexivity. Qed.
